\documentclass[a4paper, 12pt]{article}

%\usepackage[T2A]{fontenc}
\usepackage[T1]{fontenc}
\usepackage[utf8]{inputenc}
\usepackage[english]{babel}
\usepackage{amsfonts}
\usepackage{amssymb}
\usepackage{amsmath}
\usepackage{amsthm}

\begin{document}
We present classical formulas for solving quadratic, cubic and quartic equations.

\section{Quadratic equation}
Consider the equation  
\[
    ax^2+bx+c=0, \quad a\neq 0
\]
Dividing by $a$ we optain \textit{monic} equation
\[
    x^2+px+q=0
\] 
where $p=b/a,\,q=c/a$. Substitution $x=y-p/2$ will give
\[
    (y-p/2)^2+p(y-p/2)+q=y^2+q-p^2/4=0
\]
This gives
\[
    y=\pm\frac{1}{2}\sqrt{p^2-4q}
\]
Returning back to $x$:
\[
    x = -\frac{p}{2}\pm\frac{1}{2}\sqrt{p^2-4q}
\]
\section{Cubic equation}
Consider an equation
\[
    x^3+ax^2+bx+c=0
\]
Substitute $x=y-a/3$:
\[
    (y-a/3)^3+a(y-a/3)^2+b(y-a/3)+c=y^3+(b-a^2/3)y+\frac{2}{27}a^3-\frac{ab}{3}+c=0
\]
So we can solve only reduced cubic equation
\[
x^3+px+q=0    
\] 
Take $x=u+v$, then $(u+v)^3=u^3+v^3+3uv(u+v)$ and
\[
u^3+v^3+(3uv+p)(u+v)+q=0    
\]
Lets try to satisfy two conditions simultaneously
\begin{align*}
    u^3+v^3 &= -q\\
    uv &= -\frac{p}{3}
\end{align*}
It follows that $u^3$ and $v^3$ are roots of quadratic
equation 
\[
    t^2+qt-(p/3)^3=0
\]
Therefore,
\begin{align*}
    u^3 &= -\frac{q}{2}+\sqrt{(q/2)^2+(p/3)^3}\\
    v^3 &= -\frac{q}{2}-\sqrt{(q/2)^2+(p/3)^3}
\end{align*}
Finally, back to $x$:
\[
    x=\sqrt[3]{-\frac{q}{2}+\sqrt{\left(\frac{q}{2}\right)^2+\left(\frac{p}{3}\right)^3}}+\sqrt[3]{-\frac{q}{2}-\sqrt{\left(\frac{q}{2}\right)^2+\left(\frac{p}{3}\right)^3}}
\]
or 
\begin{align*}
    x&=\sqrt[3]{-\frac{q}{2}+\sqrt{D}}+\sqrt[3]{-\frac{q}{2}-\sqrt{D}}\\
    D&=\left(\frac{q}{2}\right)^2+\left(\frac{p}{3}\right)^3
\end{align*}
If $x=u+v$ is a root, then $\omega u + \omega^2 v$ and $\omega^2 u+\omega v$ are also roots, where $\omega^3=1$ is a complex cubic root of unity.
\section{Quartic equation}
Consider reduced quartic equations
\[
x^4+px^2+qx+r=0
\]
Lets find its factorization into 2 quadratic polynomials:
\[
    x^4+px^2+qx+r=(x^2+ax+b)(x^2-ax+c)
\]
Coefficients before $x$ are $a$ and $-a$ because of absent $x^3$ term.
Comparing corresponding coefficients:
\begin{align*}
    c+b &=p+a^2\\
    a(c-b) &=q\\
    bc &= r
\end{align*} 
Finding $b$ and $c$:
\begin{align*}
    2b &= p+a^2-q/a\\
    2c &= p+a^2+q/a\\
    bc &= r
\end{align*}
After substition into third equation:
\[
    (a^3+pa-q)(a^3+pa+q)=4ra^2    
\]
or
\[
    a^6+2pa^4+(p^2-4r)a^2-q^2=0
\]
Therefore we have cubic equation for $t=a^2$:
\[
t^3+2pt^2+(p^2-4r)t-q^2=0    
\]
\end{document}